feat: make implicit parameters implicit in equations
The motivation is to make "equation" notation consistent with other
notations available in Lean.

Before:
```
def Vec.map (f : α → β) : {n : Nat} → Vec α n → Vec β n
  | _, nil       => nil
  | _, cons a as => cons (f a) (map f as)
```
After:
```
def Vec.map (f : α → β) : {n : Nat} → Vec α n → Vec β n
  | nil       => nil
  | cons a as => cons (f a) (map f as)
```
If users want to pattern match on implicits, they can use a
`match-expr`.
Example:
Before:
```
protected def Path.unmap : {t : Tree α} → Path (t.map f) → Path t
  | Tree.leaf x,       Path.term _   => Path.term x
  | Tree.branch tl tr, Path.left _ _ p => Path.left tl tr (Path.unmap p)
  | Tree.branch tl tr, Path.right _ _ p => Path.right tl tr (Path.unmap p)
```
After:
```
protected def Path.unmap {t : Tree α} (p : Path (t.map f)) : Path t :=
  match t, p with
  | Tree.leaf x,   Path.term _          => Path.term x
  | Tree.branch tl tr, Path.left _ _ p  => Path.left tl tr (Path.unmap p)
  | Tree.branch tl tr, Path.right _ _ p => Path.right tl tr (Path.unmap p)

```
Another option is to use `@fun`.
```
protected def Path.unmap : {t : Tree α} → Path (t.map f) → Path t := @fun
  | Tree.leaf x,   Path.term _   => Path.term x
  | Tree.branch tl tr, Path.left _ _ p => Path.left tl tr (Path.unmap p)
  | Tree.branch tl tr, Path.right _ _ p => Path.right tl tr (Path.unmap p)
```

cc @Kha

tests/lean/run/def19.lean
@@ -1,51 +1,55 @@
 universe u
 
 inductive Vec (α : Type u) : Nat → Type u
-| nil  : Vec α 0
-| cons : α → {n : Nat} → Vec α n → Vec α (n+1)
+  | nil  : Vec α 0
+  | cons : α → {n : Nat} → Vec α n → Vec α (n+1)
 
 def Vec.append1 {α} : {m n : Nat} → Vec α m → Vec α n → Vec α (n + m)
-| _, m,  nil,      ys => ys
-| _, m, cons x xs, ys => cons x (append1 xs ys)
+  | nil,      ys => ys
+  | cons x xs, ys => cons x (append1 xs ys)
 
 def Vec.append2 {α} : {m n : Nat} → Vec α m → Vec α n → Vec α (n + m)
-| _, _,  nil,      ys => ys
-| _, _, cons x xs, ys => cons x (append2 xs ys)
+  | nil,      ys => ys
+  | cons x xs, ys => cons x (append2 xs ys)
 
-def Vec.append3 {α} : {m n : Nat} → Vec α m → Vec α n → Vec α (n + m)
-| .(_), m,  nil,      ys => ys
-| .(_), m, cons x xs, ys => cons x (append3 xs ys)
+def Vec.append3 {α} : {m n : Nat} → Vec α m → Vec α n → Vec α (n + m) :=
+  @fun
+    | .(_), m,  nil,      ys => ys
+    | .(_), m, cons x xs, ys => cons x (append3 xs ys)
 
 inductive F : Nat → Type
 | fzero : {n : Nat} → F (n+1)
 
 namespace F
 
-def fmin1 : {n : Nat} → (x y : F n) → F n
-| .(_), fzero, fzero => fzero
+def fmin1 : {n : Nat} → (x y : F n) → F n :=
+  @fun
+    | .(_), fzero, fzero => fzero
 
 def fmin2 : {n : Nat} → (x y : F n) → F n
-| _, fzero, fzero => fzero
+  | fzero, fzero => fzero
 
--- TODO: uncomment after we implement smart unfolding
--- def fmin3 : {n : Nat} → (x y : F n) → F n
--- | n+1, fzero, fzero => fzero
+def fmin3 : {n : Nat} → (x y : F n) → F n :=
+  @fun
+  | n+1, fzero, fzero => fzero
 
-def fmin4 : {n : Nat} → (x y : F n) → F n
-| .(n+1), @fzero n, @fzero .(n) => fzero
+def fmin4 : {n : Nat} → (x y : F n) → F n :=
+  @fun
+  | .(n+1), @fzero n, @fzero .(n) => fzero
 
-def fmin5 : {n : Nat} → (x y : F n) → F n
-| .(Nat.succ n), @fzero .(n), @fzero n => fzero
+def fmin5 : {n : Nat} → (x y : F n) → F n :=
+  @fun
+  | .(Nat.succ n), @fzero .(n), @fzero n => fzero
 
-def fmin6 : {n : Nat} → (x y : F n) → F n
-| .(Nat.succ _), fzero, fzero => fzero
+def fmin6 : {n : Nat} → (x y : F n) → F n :=
+  @fun
+  | .(Nat.succ _), fzero, fzero => fzero
 
 theorem ex1 (n : Nat) (x y : F n) : fmin1 x y = fmin2 x y :=
 rfl
 
--- TODO: see comment above
--- theorem ex2 (n : Nat) (x y : F n) : fmin1 x y = fmin3 x y := by
--- cases x; exact rfl
+theorem ex2 (n : Nat) (x y : F n) : fmin1 x y = fmin3 x y := by
+cases x; exact rfl
 
 theorem ex3 (n : Nat) (x y : F n) : fmin1 x y = fmin4 x y :=
 rfl
