tests/lean/223.lean
@@ -4,11 +4,11 @@ inductive Imf {α : Type u} {β : Type v} (f : α → β) : β → Type (max u v
 | mk : (a : α) → Imf f (f a)
 
 def h {α β} {f : α → β} : {b : β} → Imf f b → α
-| _, Imf.mk a => a
+| Imf.mk a => a
 
 #print h
 
-theorem ex : ∀ {α β : Sort u} (h : α = β) (a : α), cast h a ≅ a
-  | α, _, rfl, a => HEq.refl a
+theorem ex : {α β : Sort u} → (h : α = β) → (a : α) → cast h a ≅ a
+  | rfl, a => HEq.refl a
 
 #print ex
