tests/lean/run/280.lean
@@ -13,5 +13,5 @@ def Val : S → Type
   | I => Int
 
 def eval : {s : S} → Expr s → Val s
-  | _, (Expr.lit n) => n
-  | _, (Expr.eq e₁ e₂) => eval e₁ = eval e₂
+  | Expr.lit n    => n
+  | Expr.eq e₁ e₂ => eval e₁ = eval e₂
