tests/lean/run/281.lean
@@ -3,5 +3,5 @@ inductive V (α : Bool → Type) : Bool → Type
   | mk₂ : V α false → V α false
 
 def V.map {α β} (f : (b : Bool) → α b → β b) : {b : Bool} → V α b → V β b
-  | _, mk₁ x => mk₁ (f true x)
-  | _, mk₂ e => mk₂ (e.map f)
+  | mk₁ x => mk₁ (f true x)
+  | mk₂ e => mk₂ (e.map f)
