tests/lean/run/KyleAlg.lean
@@ -186,8 +186,8 @@ instance [Inv α] [Inv β] : Inv (α × β) where
 instance [One α] [One β] : One (α × β) where
     one := (1, 1)
 
-theorem Product.ext : {p q : α × β} → p.1 = q.1 → p.2 = q.2 → p = q
-    | (a, b), (c, d) => by simp; intro h; subst a; intro h; subst b; rfl
+theorem Product.ext : {p q : α × β} → p.1 = q.1 → p.2 = q.2 → p = q :=
+  @fun | (a, b), (c, d) => by simp; intro h; subst a; intro h; subst b; rfl
 
 instance [Semigroup α] [Semigroup β] : Semigroup (α × β) where
     mulAssoc := by
