tests/lean/run/def8.lean
@@ -1,5 +1,3 @@
-
-
 def g : List Nat → List Nat → Nat
 | [],         y::ys => y
 | [],         ys    => 0
@@ -13,7 +11,7 @@ inductive Imf {α : Type u} {β : Type v} (f : α → β) : β → Type (max u v
 | mk : (a : α) → Imf f (f a)
 
 def h {α β} {f : α → β} : {b : β} → Imf f b → α
-| _, Imf.mk a => a
+| Imf.mk a => a
 
 theorem ex1 {α β} (f : α → β) (a : α) : h (Imf.mk (f := f) a) = a :=
 rfl
@@ -31,13 +29,14 @@ theorem ex3 : h v₂ = 0 :=
 rfl
 
 theorem ex4 {α} : {a b : α} → a = b → b = a
-| _, _, rfl => rfl
+| rfl => rfl
 
 theorem ex5 {α} : {a b : α} → a = b → b = a
-| a, .(a), rfl => rfl
+| rfl => rfl
 
 theorem ex6 {α} : {a b : α} → a = b → b = a
-| a, .(a), Eq.refl .(a) => rfl
+| Eq.refl _ => rfl
 
-theorem ex7 {α} : {a b : α} → a = b → b = a
-| .(a), a, Eq.refl .(a) => rfl
+theorem ex7 {α} : {a b : α} → a = b → b = a :=
+ @fun
+ | .(a), a, Eq.refl .(a) => rfl
