tests/lean/run/implicitsInEqns.lean
@@ -1,0 +1,27 @@
+inductive Vec (α : Type u) : Nat → Type u
+  | nil  : Vec α 0
+  | cons : α → {n : Nat} → Vec α n → Vec α (n+1)
+
+def Nat.add' : Nat → Nat → Nat
+  | 0,      b => b
+  | succ a, b => succ (add' a b)
+
+def Vec.map (f : α → β) : {n : Nat} → Vec α n → Vec β n
+  | nil       => nil
+  | cons a as => cons (f a) (map f as)
+
+def Vec.append : {n : Nat} → Vec α n → {m : Nat} → Vec α m → Vec α (Nat.add' n m)
+  | nil,       bs => bs
+  | cons a as, bs => cons a (append as bs)
+
+def Vec.map2 (f : α → β) (as : Vec α n) : Vec β n :=
+  loop as
+where
+  loop : {n : Nat} → Vec α n → Vec β n
+    | nil       => nil
+    | cons a as => cons (f a) (loop as)
+
+def Vec.head (as : Vec α (n+1)) : α :=
+  let aux : {n : Nat} → Vec α (n+1) → α
+    | cons a _ => a
+  aux as
