tests/lean/run/renaming.lean
@@ -23,6 +23,6 @@ def liftr {g d a} (r : Ren g d) : Ren (a :: g) (a :: d)
   | _, Var.vs x => Var.vs (r _ x)
 
 def rename {g d : Cxt} : (r : Ren g d) → {a : Ty} → Term d a → Term g a
-  | r, _, Term.var x   => Term.var (r _ x)
-  | r, _, Term.app t u => Term.app (rename r t) (rename r u)
-  | r, _, Term.abs t   => Term.abs (rename (liftr r) t)
+  | r, Term.var x   => Term.var (r _ x)
+  | r, Term.app t u => Term.app (rename r t) (rename r u)
+  | r, Term.abs t   => Term.abs (rename (liftr r) t)
